Ackermann.v
@@ -1,32 +1,38 @@
+Add LoadPath "/home/user/0my/GITHUB/VerifiedMathFoundations/library".
 Require List.
 Require Bool.
 Require Import Coq.Structures.Equalities.
-Add LoadPath "/home/user/0my/GITHUB/VerifiedMathFoundations/library".
 Require Export Provability.
 
-Module Ackermann_mod (*SetVars FuncSymb PredSymb: UsualDecidableTypeFull*).
-Module SetVars := PeanoNat.Nat.
-Module FuncSymb := PeanoNat.Nat.
-Module PredSymb := PeanoNat.Nat.
-Module X := Provability_mod SetVars FuncSymb PredSymb.
-Export X.
 Export Coq.Lists.List.
 Import Bool.Bool.
 
-(*Notation SetVars := SetVars.t (*only parsing*).
-Notation FuncSymb := FuncSymb.t (only parsing).
-Notation PredSymb := PredSymb.t (*only parsing*).*)
+Module Ackermann_mod (*SetVars FuncSymb PredSymb: UsualDecidableTypeFull*).
+Module SetVars : UsualDecidableTypeFull :=PeanoNat.Nat.
+Module FuncSymb : UsualDecidableTypeFull := PeanoNat.Nat.
+Module PredSymb : UsualDecidableTypeFull := PeanoNat.Nat.
+
+Module X := Provability_mod SetVars FuncSymb PredSymb.
+Export X.
+Module Facts := BoolEqualityFacts SetVars.
 Check substF.
+
+(*Local Notation SetVars := SetVars.t (only parsing).
+Local Notation FuncSymb := FuncSymb.t (only parsing).
+Local Notation PredSymb := PredSymb.t (only parsing). *)
+
 Import VectorNotations.
 (*Check substF.*)
 
+Section inf_sec.
+Context (en:nat->PredSymb.t) (enInj: forall x1 x2, en x1 = en x2 -> x1=x2).
 (*Module Facts := BoolEqualityFacts SetVars.*)
 Inductive AxiomAST : Fo -> Type :=
 | aPC  :> forall {A}, (AxiomH A) -> (AxiomAST A)
-| aeq1 : forall (x:SetVars), (AxiomAST (Atom (MPSV 0 2) [FVC x ; FVC x]))
-| aeq2 : forall (x y:SetVars) (f r:Fo) 
-(*H: substF y *)
-, (AxiomAST (Atom (MPSV 0 1) [FVC x] ))
+| aeq1 : forall (x:SetVars.t), (AxiomAST (Atom (MPSV (en 0) 2) [FVC x ; FVC x]))
+| aeq2 : forall (x y:SetVars.t) (f r:Fo)
+(H:substF y x f = Some r)
+, (AxiomAST (Atom (MPSV (en 0) 2) [FVC x ; FVC y] --> ( r --> f) ))
 .
 
 (* (MPSV 0 2) - = 
@@ -34,11 +40,32 @@ Inductive AxiomAST : Fo -> Type :=
 *)
 (*Check AxiomAST (Ha1 Bot Bot). ? *)
 
-
+Notation "( a '==' b )" := (Atom (MPSV (en 0) 2) [a ; b]).
+Notation "( a 'e.' b )" := (Atom (MPSV (en 1) 2) [a ; b]).
 
 (* Provability in Ackermann set theory *)
 Definition APR := @GPR AxiomAST.
+(* Mendelson p.102/447 *)
+(*Coercion FVC : SetVars.t >-> Terms.*)
+(*Coercion Q : (Vector.t SetVars.t n) >-> (Vector.t Terms n).*)
 
+Definition p2_23_a ctx (t:Terms) (x:SetVars.t): 
+APR ctx (Atom (MPSV (en 0) 2) [t ; t]).
+Proof. (* (Atom (MPSV (en 0) 2) [FVC x ; FVC x]) *)
+apply MP with (A:= Fora x (FVC x== FVC x)).
+apply GEN.
+apply Hax, (aeq1 x).
+apply Hax, aPC.
+apply Ha12 with (t:=t).
+simpl.
+rewrite -> Facts.eqb_refl.
+reflexivity.
+Defined.
+Definition p2_23_b ctx (t s:Terms) (x:SetVars.t): 
+APR ctx ((Atom (MPSV (en 0) 2) [t ; t]) --> (Atom (MPSV (en 0) 2) [t ; t]) ).
+Proof.
 
+Abort.
+End inf_sec.
 
 End Ackermann_mod.
