Provability.v
@@ -9,11 +9,11 @@ Module Provability_mod (SetVars FuncSymb PredSymb: UsualDecidableTypeFull).
 Module XPro := Formulas.Formulas_mod SetVars FuncSymb PredSymb.
 Export XPro.
 
-(*
-Notation SetVars := SetVars.t (only parsing).
-Notation FuncSymb := FuncSymb.t (only parsing).
-Notation PredSymb := PredSymb.t (only parsing).
-*)
+
+(*Local Notation SetVars := SetVars.t (*only parsing*).
+Local Notation FuncSymb := FuncSymb.t (*only parsing*). 
+Local Notation PredSymb := PredSymb.t (*only parsing*).*)
+
 (*Notation " x --> y ":=(Impl x y) (at level 80).*)
 
 (*Open Scope list_scope.*)
@@ -27,9 +27,9 @@ fix InL (a : A) (l : list A) {struct l} : Type :=
 Inductive AxiomH : Fo -> Type :=
 | Ha1  : forall A B, AxiomH (A-->(B-->A))
 | Ha2  : forall A B C, AxiomH ((A-->(B-->C))-->((A-->B)-->(A-->C)))
-| Ha12 : forall (ph: Fo) (t:Terms) (xi:SetVars)
+| Ha12 : forall (ph: Fo) (t:Terms) (xi:SetVars.t)
  (r:Fo) (s:(substF t xi ph)=Some r), AxiomH (Impl (Fora xi ph) r)
-| Hb1  : forall (ps ph: Fo) (xi:SetVars) (H:isParamF xi ps = false),
+| Hb1  : forall (ps ph: Fo) (xi:SetVars.t) (H:isParamF xi ps = false),
 AxiomH (Impl (Fora xi (Impl ps ph)) (Impl ps (Fora xi ph)) )
 .
 
@@ -38,7 +38,7 @@ Inductive GPR {axs : Fo -> Type} (ctx:list Fo) : Fo -> Type :=
 | Hax (A : Fo): (axs A) -> @GPR axs ctx A
 | MP (A B: Fo) : (@GPR axs ctx A)->(@GPR axs ctx (Impl A B))
                  ->(@GPR axs ctx B)
-| GEN (A : Fo) (xi:SetVars): (@GPR axs ctx A)->(@GPR axs ctx (Fora xi A))
+| GEN (A : Fo) (xi:SetVars.t): (@GPR axs ctx A)->(@GPR axs ctx (Fora xi A))
 .
 
 (* Provability in predicate calculus *)
@@ -64,7 +64,7 @@ Definition a1 axi A B : @PR axi (Impl A (Impl B A)).
 Proof. apply Hax, Ha1. Defined.
 Definition a2 axi A B C : @PR axi ((A-->(B-->C))-->((A-->B)-->(A-->C))).
 Proof. apply Hax, Ha2. Defined.
-Definition b1 axi (ps ph: Fo) (xi:SetVars) (H:isParamF xi ps = false):
+Definition b1 axi (ps ph: Fo) (xi:SetVars.t) (H:isParamF xi ps = false):
 @PR axi (Impl (Fora xi (Impl ps ph)) (Impl ps (Fora xi ph)) ).
 Proof. apply Hax, Hb1, H. Defined.
 
